Migrate HReduce and Softmax to Array1
No dist diff. But several admits added due to needing memcpy.

src/lib/data/Kuiper.Array1.fst
@@ -19,9 +19,23 @@ let abs_bij (#len : nat) : (abs (desc len) =~ ait len) =
 let tr_val (#et : Type) (#len : nat) (s : lseq et len) : chest (desc len) et =
   Chest.mk (desc len) (fun (i, ()) -> s @! i)
 
+let backtr_val (#et : Type) (#len : nat) (c : chest (desc len) et) : GTot (lseq et len) =
+  Seq.init_ghost len (fun i -> Chest.acc c (i, ()))
+
 inline_for_extraction noextract
 let adapt_cit_back (len : erased nat) (idx : raw_cit{cit_fits len idx}) : conc (desc len) =
   (idx, ())
+
+let to_from (#et:Type) (#len : nat) (l : full_layout len) (s : lseq et len)
+  : Lemma (to_seq l (from_seq l s) == s)
+          [SMTPat (to_seq l (from_seq l s))]
+  = let aux (i : natlt len) : Lemma (to_seq l (from_seq l s) @! i == Seq.index s i) =
+      ()
+    in
+    // ^ Why is this needed?
+    Classical.forall_intro aux;
+    assert (Seq.equal (to_seq l (from_seq l s)) s);
+    ()
 
 let t (et : Type0) (#len : nat) (l : layout len) : Type0 =
   T.tensor et l
@@ -82,6 +96,47 @@ instance is_send_across_global
   (#f : perm) (s : lseq et len)
   : is_send_across gpu_of (pts_to a #f s)
   = solve
+
+inline_for_extraction noextract
+fn alloc0
+  (#et:Type) {| sized et |}
+  (len : szp)
+  (l : layout len { is_full l })
+  preserves
+    cpu
+  returns
+    p : t et l
+  ensures
+    exists* em. on gpu_loc (p |-> em)
+  ensures
+    pure (is_global p)
+{
+  let t = T.alloc0 #et len l;
+  with em. assert on gpu_loc (T.tensor_pts_to t em);
+  assert pure (Chest.equal em (tr_val (backtr_val em)));
+  rewrite on gpu_loc (T.tensor_pts_to t em)
+       as on gpu_loc (pts_to t (backtr_val em));
+  t
+}
+
+inline_for_extraction noextract
+fn free
+  (#et:Type)
+  (#len : erased nat)
+  (#l : layout len { is_full l })
+  (p : t et l)
+  (#em : erased (lseq et len))
+  preserves
+    cpu
+  requires
+    on gpu_loc (p |-> em)
+  ensures
+    emp
+{
+  rewrite on gpu_loc (pts_to p em)
+       as on gpu_loc (T.tensor_pts_to p (tr_val em));
+  T.free p;
+}
 
 ghost
 fn pts_to_ref
@@ -231,4 +286,164 @@ fn implode
   forevery_ext _ (fun (i : abs (desc len)) -> Cell a i |-> Frac f (acc (tr_val s) i));
   T.tensor_implode a;
   fold pts_to a #f s;
+}
+
+inline_for_extraction noextract
+fn read_cell
+  (#et : Type0) (#len : erased nat)
+  (#l : layout len ) {| ctlayout l |}
+  (a : t et l)
+  (i : raw_cit{cit_fits len i})
+  (#f : perm)
+  (#s : erased et)
+  preserves
+    Cell a (i <: natlt len) |-> Frac f s
+  returns
+    v : et
+  ensures
+    pure (v == s)
+{
+  unfold pts_to_cell a #f i s;
+  let v = T.tensor_read_cell a (adapt_cit_back len i);
+  fold pts_to_cell a #f i s;
+  v
+}
+
+inline_for_extraction noextract
+fn write_cell
+  (#et : Type0) (#len : erased nat)
+  (#l : layout len ) {| ctlayout l |}
+  (a : t et l)
+  (i : raw_cit{cit_fits len i})
+  (v : et)
+  (#s : erased et)
+  requires
+    Cell a (i <: natlt len) |-> s
+  ensures
+    Cell a (i <: natlt len) |-> v
+{
+  unfold pts_to_cell a i s;
+  T.tensor_write_cell a (adapt_cit_back len i) v;
+  fold pts_to_cell a i v;
+}
+
+inline_for_extraction noextract
+fn memcpy_host_to_device
+  (#et:Type) {| sized et |} (#len : erased nat) (#l : full_layout len)
+  (dst : t et l) (src : vec et) (n : sz)
+  (#vsrc : erased (lseq et len))
+  (#vdst : erased (lseq et len))
+  preserves
+    cpu
+  preserves
+    src |-> vsrc
+  requires
+    pure (SZ.v n == len)
+  requires
+    on gpu_loc (dst |-> vdst)
+  ensures
+    on gpu_loc (dst |-> from_seq l vsrc)
+{
+  (* Should be proven. *)
+  map_loc gpu_loc
+    #(dst |-> vdst)
+    #(core dst |-> to_seq l vdst)
+    fn _ { admit(); };
+
+  gpu_memcpy_host_to_device (core dst) src n;
+
+  (* Should be proven. *)
+  map_loc gpu_loc
+    #(core dst |-> vsrc)
+    #(dst |-> from_seq l vsrc)
+    fn _ { admit(); };
+  ();
+}
+
+inline_for_extraction noextract
+fn memcpy_device_to_host'
+  (#a:Type u#0)
+  {| sized a |}
+  (#dst_sz : erased nat)
+  (dst_arr : vec a)
+  (dst_off : SZ.t)
+  (#src_sz : erased nat)
+  (src : t a (Kuiper.Tensor.Layout.Alg.l1_forward src_sz))
+  (src_off : SZ.t)
+  (cnt : SZ.t {
+    dst_off + cnt <= dst_sz /\
+          src_off + cnt <= src_sz
+  })
+  (#f : perm)
+  (#v : erased (lseq a src_sz))
+  (#gv : erased (lseq a dst_sz))
+  preserves
+    cpu **
+    on gpu_loc (src |-> Frac f v)
+  requires
+    dst_arr |-> gv
+  ensures
+    exists* (s' : lseq a dst_sz).
+      dst_arr |-> s' **
+      pure (s' == Kuiper.Seq.Common.seq_blit gv dst_off v src_off cnt)
+{
+  (* Should prove *)
+  map_loc gpu_loc
+    #(src |-> Frac f v)
+    #(core src |-> Frac f v)
+    fn _ { admit(); };
+
+  (* Bulk copy at the gpu_array level *)
+  gpu_memcpy_device_to_host' #_ #_ #dst_sz dst_arr dst_off #_ (core src) src_off cnt;
+
+  (* Should prove *)
+  map_loc gpu_loc
+    #(core src |-> Frac f v)
+    #(src |-> Frac f v)
+    fn _ { admit(); };
+  ()
+}
+
+inline_for_extraction noextract
+fn memcpy_device_to_device
+  (#a:Type u#0)
+  {| sized a |}
+  (#sz : erased nat)
+  (#l : full_layout sz)
+  (dst : t a l)
+  (src : t a l)
+  (cnt : SZ.t)
+  (#f : perm)
+  (#vsrc #vdst : erased (lseq a sz))
+  preserves
+    cpu **
+    on gpu_loc (src |-> Frac f vsrc)
+  requires
+    on gpu_loc (dst |-> vdst) **
+    pure (SZ.v cnt == sz)
+  ensures
+    on gpu_loc (dst |-> vsrc)
+{
+  (* Should be proven. *)
+  map_loc gpu_loc
+    #(dst |-> vdst)
+    #(core dst |-> to_seq l vdst)
+    fn _ { admit(); };
+  map_loc gpu_loc
+    #(src |-> Frac f vsrc)
+    #(core src |-> Frac f (to_seq l vsrc))
+    fn _ { admit(); };
+
+  gpu_memcpy_device_to_device (core dst) (core src) cnt;
+
+  (* Should be proven. *)
+  map_loc gpu_loc
+    #(core src |-> Frac f (to_seq l vsrc))
+    #(src |-> Frac f vsrc)
+    fn _ { admit(); };
+  map_loc gpu_loc
+    #(core dst |-> to_seq l vsrc)
+    #(dst |-> vsrc)
+    fn _ { admit(); };
+  ();
 }
