src/lib/poly/Kuiper.Poly.DotProduct.fsti
@@ -28,17 +28,14 @@ type dotprod_ty
   fn (lena : szp{lena <= max_threads})
      (a1 : vec et)
      (a2 : vec et)
-     (v1 : erased (seq et))
-     (v2 : erased (seq et))
-     (vr1 : erased (seq real))
-     (vr2 : erased (seq real) {seq_approximates v1 vr1 /\ seq_approximates v2 vr2})
-     (#_: squash (len v1 == SZ.v lena /\ len v2 == SZ.v lena))
+     (#v1 #v2 : erased (lseq et lena))
+     (vr1 vr2: erased (lseq real lena) { v1 %~ vr1 /\ v2 %~ vr2 })
   preserves
     cpu ** a1 |-> v1 ** a2 |-> v2
   returns
     dp : et
   ensures
-    pure (dp `approximates` sum (pmul vr1 vr2))
+    pure (dp %~ sum (pmul vr1 vr2))
 
 inline_for_extraction noextract
 val dotprod
